Axiom.lean
@@ -5,3 +5,4 @@ import Axiom.Save
 import Axiom.Render
 import Axiom.Audio
 import Axiom.Effects
+import Axiom.Theorems
